

Exercises

Tail Recursive Functions

Exercise 1:

In the previous exercise set, you wrote the code for:

```
fibonacci :: Int -> Int
```

that calculates the Fibonacci number as per the following definition (note for non-negative integers)

$$F_0 = 0, F_1 = 1$$

$$F_n = F_{n-1} + F_{n-2}$$

Now, write this fibonacci using tail recursion.

```
fibT :: Int -> Int
```

Solution 1:

```
fibT :: Int -> Int
```

```
fibT n = helper n 1 0 where
```

```
    helper 1 prev prevBut1 = prev
```

```
    helper n prev prevBut1 = helper (n-1) (prev+prevBut1) prev
```

Exercise 2:

Noting our definition of add from the previous lecture (this is actually tail recursive)

```
myAdd :: Int -> Int -> Int
```

```
myAdd x 0 = x
```

```
myAdd 0 y = y
```

```
myAdd x y = myAdd (x-1) (y+1)
```

write a function

```
myMult :: Int -> Int -> Int
```

which takes two positive integers and returns the product of the two numbers. This calculation can only use + and -. Ensure that the solution is tail recursive

Solution 2:

non-tail recursive:

```
recMult :: Int -> Int -> Int
```

```
recMult x 1 = x
```

```
recMult 1 y = y
```

```
recMult x y = x + recMult x (y-1)
```

and using tail recursion:

```
tailMult :: Int -> Int -> Int
tailMult x y = helperMult x y 0
where helperMult x y acc
      | y == 0 = acc
      | otherwise = helperMult x (y-1) (acc+x)
```

Exercise 3:

Given the recursive function

```
reverse_ :: [a] -> [a]
reverse_ [] = []
reverse_ (x:xs) = reverse_ xs ++ [x]
```

that returns the reverse of a list, but this time, using tail recursion.

Solution 3:

```
reverseAccum :: [a] -> [a]
reverseAccum list = revHelper [] list
      where revHelper accum [] = accum
           revHelper accum (x:xs) = revHelper (x:accum) xs
```